interp_state preserves sbisim
for simple enough handlers

theories/Interp/State.v
@@ -121,6 +121,14 @@ Section State.
     rewrite unfold_interp_state; reflexivity.
   Qed.
 
+  Lemma interp_state_choice {E F : Type -> Type} {T : Type}
+        (b : bool) (n : nat) (k : fin n -> ctree E T) (h : E ~> stateT S (ctree F)) (s : S)
+    : interp_state h (Choice b n k) s
+                   ≅ Choice b n (fun sx => TauI (interp_state h (k sx) s)).
+  Proof.
+    rewrite unfold_interp_state; reflexivity.
+  Qed.
+
   Lemma interp_state_tau {E F : Type -> Type} {T : Type}
         (t : ctree E T) (h : E ~> Monads.stateT S (ctree F)) (s : S)
     : interp_state h (TauI t) s ≅ TauI (TauI (interp_state h t s)).
@@ -186,6 +194,357 @@ Section State.
       step; constructor; intros ?.
       apply IH.
   Qed.
+
+Lemma trans0_interp_state : forall {E F X} (h : E ~> stateT S (ctree F)) (t t' : ctree E X) s,
+  trans0 t t' -> trans0 (interp_state h t s) (interp_state h t' s).
+Proof.
+  intros. red in H. setoid_rewrite (ctree_eta t). setoid_rewrite (ctree_eta t').
+  genobs t ot. genobs t' ot'. clear t Heqot t' Heqot'.
+  induction H.
+  - constructor. rewrite H. reflexivity.
+  - rewrite unfold_interp_state. cbn.
+    apply T0Choice with (x := x).
+    apply T0Choice with (x := Fin.F1). apply IHtrans0_.
+Qed.
+
+(* transi *)
+
+Inductive transi_state {E F X} (h : E ~> stateT S (ctree F)) : @label F -> S -> S -> ctree E X -> ctree E X -> Prop :=
+| transis_val : forall (x : X) t t' s,
+    trans (val x) t t' ->
+    transi_state h (val (s, x)) s s t t'
+| transis_tau : forall t t' s,
+    trans tau t t' ->
+    transi_state h tau s s t t'
+| transis_obs : forall Y (e : E Y) x l t t' t'' s s',
+    trans (obs e x) t t' ->
+    t0_det t'' (Ret (s', x)) ->
+    trans l (h _ e s) t'' ->
+    transi_state h l s s' t t'
+| transis_obs0 : forall Y (e : E Y) l x t t' t'' s s' s'',
+    trans (obs e x) t t' ->
+    transi_state h l s' s'' t' t'' ->
+    trans (val (s', x)) (h _ e s) CTree.stuckI ->
+    transi_state h l s s'' t t''
+.
+
+#[global] Instance transis_equ :
+  forall {E F X} (h : E ~> stateT S (ctree F)) l s s',
+  Proper (equ eq ==> equ eq ==> flip impl) (@transi_state E F X h l s s').
+Proof.
+  cbn. intros.
+  revert x x0 H H0. induction H1; intros.
+  - apply transis_val. rewrite H0, H1. apply H.
+  - apply transis_tau. rewrite H0, H1. apply H.
+  - rewrite <- H2, <- H3 in *. eapply transis_obs; eauto.
+  - rewrite <- H2 in *. eapply transis_obs0; eauto.
+Qed.
+
+#[global] Instance transis_equ' :
+  forall {E F X} (h : E ~> stateT S (ctree F)) l s s',
+  Proper (equ eq ==> equ eq ==> impl) (@transi_state E F X h l s s').
+Proof.
+  cbn. intros. rewrite <- H, <- H0. apply H1.
+Qed.
+
+Lemma transis_choiceI {E F X} (h : E ~> stateT S (ctree F)) : forall l s s' (t' : ctree E X) n k x,
+  transi_state h l s s' (k x) t' ->
+  transi_state h l s s' (ChoiceI n k) t'.
+Proof.
+  intros. inv H.
+  - apply transis_val. etrans.
+  - apply transis_tau. etrans.
+  - eapply transis_obs; etrans.
+  - eapply transis_obs0; etrans.
+Qed.
+
+Lemma trans0_transi {E F X} (h : E ~> stateT S (ctree F)) :
+  forall l s s' (t t' t'' : ctree E X), trans0 t t' -> transi_state h l s s' t' t'' -> transi_state h l s s' t t''.
+Proof.
+  intros.
+  red in H. rewrite (ctree_eta t). rewrite (ctree_eta t') in H0.
+  genobs t ot. genobs t' ot'. clear t Heqot. clear t' Heqot'.
+  revert l t'' H0. induction H; intros.
+  - rewrite H. apply H0.
+  - eapply transis_choiceI. setoid_rewrite <- ctree_eta in IHtrans0_. apply IHtrans0_. apply H0.
+Qed.
+
+Lemma transis_sbisim {E F X} (h : E ~> stateT S (ctree F)) :
+  forall l s s' (t t' u : ctree E X), transi_state h l s s' t t' ->
+  t ~ u ->
+  exists u', transi_state h l s s' u u' /\ t' ~ u'.
+Proof.
+  intros. revert u H0.
+  induction H; intros.
+  - step in H0. destruct H0 as [? _]. apply H0 in H. destruct H.
+    exists x0. split. now apply transis_val. apply H1.
+  - step in H0. destruct H0 as [? _]. apply H0 in H. destruct H.
+    exists x. split. now apply transis_tau. apply H1.
+  - step in H2. destruct H2 as [? _]. apply H2 in H. destruct H.
+    exists x0. split. eapply transis_obs; eauto. apply H3.
+  - step in H2. destruct H2 as [? _]. apply H2 in H. destruct H.
+    apply IHtransi_state in H3 as (? & ? & ?). exists x1.
+    split. eapply transis_obs0; eauto. apply H4.
+Qed.
+
+Lemma transis_trans {E F X} (h : E ~> stateT S (ctree F)) (Hh : forall X e s, vsimple (h X e s)) :
+  forall l s s' (t t' : ctree E X),
+  transi_state h l s s' t t' -> exists t0, trans l (interp_state h t s) t0 /\ t0_det t0 (interp_state h t' s').
+Proof.
+  intros. induction H.
+  - exists CTree.stuckI. apply trans_val_inv in H as ?.
+    apply trans_val_trans0 in H as [].
+    eapply trans0_interp_state in H. rewrite interp_state_ret in H. setoid_rewrite H0.
+    setoid_rewrite interp_state_choice. setoid_rewrite choice0_always_stuck.
+    eapply trans0_trans in H; etrans. split; etrans. now left.
+  - exists (TauI (interp_state h t' s)). split; [| eright; eauto; now left ].
+    apply trans_tau_trans0 in H as (? & ? & ? & ? & ?).
+    eapply trans0_interp_state in H. setoid_rewrite H0. eapply trans0_trans; etrans.
+    setoid_rewrite interp_state_choice.
+    econstructor. reflexivity.
+  - exists (x <- t'';; TauI (interp_state h t' s')).
+    split. 2: { eapply t0_det_bind_ret_l; eauto. eright; eauto. now left. }
+    apply trans_obs_trans0 in H as (? & ? & ?).
+    eapply trans0_interp_state in H. setoid_rewrite H2. eapply trans0_trans; etrans.
+    setoid_rewrite interp_state_vis.
+    eapply trans_bind_l with (k := fun sx => TauI (interp_state h (x0 (snd sx)) (fst sx))) in H1.
+    setoid_rewrite t0_det_bind_ret_l_equ in H1 at 2; eauto. cbn in *. eapply H1.
+    { intro. inv H3. apply trans_val_inv in H1. rewrite H1 in H0. inv H0. step in H3. inv H3. step in H4. inv H4. }
+  - destruct IHtransi_state as (? & ? & ?).
+    destruct (Hh Y e s). 2: { destruct H4. rewrite H4 in H1. apply trans_vis_inv in H1 as (? & ? & ?). step in H1. inv H1. }
+    destruct H4. rewrite H4 in H1. inv_trans. subst.
+    exists x0. split. 2: auto.
+    apply trans_obs_trans0 in H as (? & ? & ?). eapply trans0_interp_state in H.
+    setoid_rewrite interp_state_vis in H. setoid_rewrite H4 in H. setoid_rewrite bind_ret_l in H.
+    eapply trans0_trans; etrans. setoid_rewrite <- H1. etrans.
+Qed.
+
+(** Various lemmas for the proof that interp_state preserves sbisim in some cases. *)
+
+Lemma interp_state_ret_inv {E F X} (h : E ~> stateT S (ctree F)) : forall s (t : ctree E X) r,
+  interp_state h t s ≅ Ret r -> t ≅ Ret (snd r) /\ s = fst r.
+Proof.
+  intros. setoid_rewrite (ctree_eta t) in H. setoid_rewrite (ctree_eta t).
+  destruct (observe t) eqn:?.
+  - rewrite interp_state_ret in H. step in H. inv H. split; reflexivity.
+  - rewrite interp_state_vis in H. apply ret_equ_bind in H as (? & ? & ?). step in H0. inv H0.
+  - rewrite interp_state_choice in H. step in H. inv H.
+Qed.
+
+Lemma trans_interp_state_inv_gen {E F X Y} (h : E ~> stateT S (ctree F)) (Hh : forall X e s, vsimple (h X e s)) :
+  forall l s (k : Y -> ctree E X) t' (pre : ctree F Y),
+  is_simple pre ->
+  trans l (x <- pre;; interp_state h (k x) s) t' ->
+  exists t0 s', t0_det t' (interp_state h t0 s') /\
+  ((exists l t1 x, trans l pre t1 /\ t0_det t1 (Ret x : ctree F Y) /\ t0 ≅ k x) \/
+    exists (x : Y), trans (val x) pre CTree.stuckI /\ trans l (interp_state h (k x) s) t' /\ transi_state h l s s' (k x) t0).
+Proof.
+  intros * Hpre H.
+  do 3 red in H. remember (observe (x <- pre;; interp_state h (k x) s)) as oi.
+  setoid_rewrite (ctree_eta t') at 1.
+  setoid_rewrite (ctree_eta t') at 2.
+  genobs t' ot'. clear t' Heqot'.
+  assert (go oi ≅ x <- pre;; interp_state h (k x) s).
+  { rewrite Heqoi, <- ctree_eta. reflexivity. } clear Heqoi.
+  revert Y s k pre Hpre H0. induction H; intros.
+  - destruct n. now apply Fin.case0.
+    symmetry in H0. apply choice_equ_bind in H0 as ?.
+    destruct H1 as [[] | (? & ? & ?)].
+    + rewrite H1 in H0. setoid_rewrite bind_ret_l in H0. setoid_rewrite H1. clear pre Hpre H1.
+      rewrite (ctree_eta (k0 x0)) in H0. destruct (observe (k0 x0)) eqn:?.
+      * rewrite interp_state_ret in H0. step in H0. inv H0.
+      * rewrite interp_state_vis in H0. apply choice_equ_bind in H0 as ?. destruct H1 as [[] | (? & ? & ?)].
+        --setoid_rewrite H1 in H0. setoid_rewrite bind_ret_l in H0.
+          apply equ_choice_invT in H0 as ?. destruct H2 as [? _]. apply eq_add_S in H2 as <-.
+          simple apply equ_choice_invE with (x := x) in H0.
+          rewrite <- H0 in H.
+          specialize (IHtrans_ _ (fst x1) (fun (_ : unit) => k1 (snd x1)) (Ret tt)).
+          edestruct IHtrans_ as (? & ? & ?).
+          { apply is_simple_ret. }
+          { rewrite <- ctree_eta. setoid_rewrite bind_ret_l. setoid_rewrite H0. reflexivity. }
+          destruct H2. exists x2, x3. split; auto. right. destruct H3.
+          { destruct H3 as (? & ? & ? & ? & ? & ?). inv_trans. subst.
+            inv H4. step in H3. inv H3. step in H6. inv H6. }
+          destruct H3 as (_ & _ & ? & ?). exists x0. split. etrans. split.
+          ++setoid_rewrite (ctree_eta (k0 x0)). rewrite Heqc.
+            setoid_rewrite interp_state_vis. setoid_rewrite H1. setoid_rewrite bind_ret_l. apply trans_tauI. apply H3.
+          ++setoid_rewrite (ctree_eta (k0 x0)). rewrite Heqc. destruct x1.
+             eapply transis_obs0. etrans. 2: { rewrite H1. etrans. } cbn in H4. cbn in *. etrans.
+        --destruct (Hh X0 e s).
+          destruct H3. rewrite H3 in H1. step in H1. inv H1.
+          destruct H3. rewrite H3 in H1. step in H1. inv H1.
+      * rewrite interp_state_choice in H0.
+        apply equ_choice_invT in H0 as ?. destruct H1 as [-> ->].
+        simple apply equ_choice_invE with (x := x) in H0 as ?.
+        specialize (IHtrans_ _ s (fun _ : unit => k1 x) (TauI (Ret tt))).
+        edestruct IHtrans_ as (? & ? & ? & ?).
+        { apply is_simple_tauI_ret. }
+        { rewrite <- ctree_eta. setoid_rewrite bind_choice. setoid_rewrite bind_ret_l. now rewrite H1. }
+        destruct H3.
+        { destruct H3 as (? & ? & ? & ? & ? & ?). inv_trans. subst.
+          inv H4. step in H3. inv H3. step in H5. inv H5. }
+        destruct H3 as (? & ? & ? & ?).
+        exists x1, x2. split; auto. right. exists x0. split; etrans. split.
+        rewrite (ctree_eta (k0 x0)), Heqc, interp_state_choice.
+        eapply trans_choiceI. 2: reflexivity. apply trans_tauI. apply H4.
+        rewrite (ctree_eta (k0 x0)), Heqc. eapply transis_choiceI; etrans.
+    + specialize (IHtrans_ _ s k0 (x0 x)).
+      edestruct IHtrans_ as (? & ? & ? & ?).
+      { apply is_simple_choiceI. red. setoid_rewrite <- H1. apply Hpre. }
+      rewrite <- ctree_eta. apply H2. destruct H4 as [(? & ? & ? & ? & ? & ?) | (? & ? & ? & ?)].
+        exists (k0 x5), x2. split. { now rewrite H6 in H3. }
+        left. eapply trans_choiceI in H4. 2: reflexivity. rewrite <- H1 in H4. eauto 6.
+      * exists x1, x2. split; auto. right. exists x3. rewrite H1. etrans.
+  - destruct n. now apply Fin.case0.
+    symmetry in H0. apply choice_equ_bind in H0 as ?. destruct H1 as [[] | (? & ? & ?)].
+    + rewrite H1 in H0. setoid_rewrite bind_ret_l in H0.
+      rewrite (ctree_eta (k0 x0)) in H0. destruct (observe (k0 x0)) eqn:?.
+      * rewrite interp_state_ret in H0. step in H0. inv H0.
+      * rewrite interp_state_vis in H0. apply choice_equ_bind in H0 as ?.
+        destruct H2 as [[] | (? & ? & ?)].
+        { rewrite H2 in H0. setoid_rewrite bind_ret_l in H0. step in H0. inv H0. }
+        pose proof (trans_choiceV x1 x). rewrite <- H2 in H4.
+        edestruct Hh. { destruct H5. rewrite H5 in H4. inv_trans. }
+        destruct H5. rewrite H5 in H4. apply trans_vis_inv in H4 as (? & ? & ?). discriminate.
+      * rewrite interp_state_choice in H0.
+        apply equ_choice_invT in H0 as ?. destruct H2 as [-> ->].
+        simple eapply equ_choice_invE in H0 as ?. rewrite H in H2.
+        exists (k1 x), s. symmetry in H2. split.
+        { rewrite <- ctree_eta. rewrite H2. eapply t0_det_tau; auto. apply t0_det_id; auto. }
+        right. exists x0. rewrite H1. split; etrans.
+        split; setoid_rewrite (ctree_eta (k0 x0)); setoid_rewrite Heqc.
+        { setoid_rewrite interp_state_choice. rewrite H2.
+          econstructor. now rewrite <- ctree_eta. }
+        econstructor; etrans.
+    + pose proof (trans_choiceV x0 x).
+      rewrite <- H1 in H3. edestruct Hpre.
+      { apply H4 in H3. inv H3. }
+      apply H4 in H3 as [].
+      specialize (H2 x).
+      exists (k0 x1), s. rewrite H in H2. split.
+      { rewrite <- ctree_eta, H2. eapply t0_det_bind_ret_l; eauto. now left. }
+      left. exists tau, (x0 x), x1. split; auto. rewrite H1. etrans.
+  - symmetry in H0. apply vis_equ_bind in H0 as ?. destruct H1 as [[] | (? & ? & ?)].
+    + rewrite H1 in H0. setoid_rewrite bind_ret_l in H0.
+     rewrite (ctree_eta (k0 x0)) in H0. destruct (observe (k0 x0)) eqn:?.
+      * rewrite interp_state_ret in H0. step in H0. inv H0.
+      * rewrite interp_state_vis in H0. apply vis_equ_bind in H0 as ?.
+        destruct H2 as [[] | (? & ? & ?)].
+        { rewrite H2 in H0. setoid_rewrite bind_ret_l in H0. step in H0. inv H0. }
+        pose proof (trans_vis e x x1). rewrite <- H2 in H4.
+        edestruct Hh. { destruct H5. rewrite H5 in H4. inv H4. }
+        destruct H5. rewrite H5 in H4.
+        specialize (H3 x). rewrite H5 in H2.
+        apply equ_vis_invT in H2 as ?. subst.
+        apply equ_vis_invE in H2 as ?. destruct H6 as [-> ?].
+        rewrite <- H6 in *. rewrite bind_ret_l in H3.
+        exists (k1 (snd x)), (fst x).
+        rewrite H in H3. split. { rewrite <- ctree_eta, H3. eright; eauto. eleft; auto. }
+        right.
+        exists x0. rewrite H1. split; etrans.
+        split; setoid_rewrite (ctree_eta (k0 x0)); setoid_rewrite Heqc.
+        { setoid_rewrite interp_state_vis. rewrite H5. setoid_rewrite bind_vis.
+          econstructor. rewrite bind_ret_l. rewrite <- H3, <- ctree_eta. reflexivity. }
+        eapply transis_obs; etrans. 2: { rewrite H5. etrans. } destruct x. now left.
+      * rewrite interp_state_choice in H0. step in H0. inv H0.
+    + pose proof (trans_vis e x x0).
+      rewrite <- H1 in H3. edestruct Hpre.
+      { apply H4 in H3. inv H3. }
+      apply H4 in H3 as [].
+      specialize (H2 x).
+      exists (k0 x1), s. rewrite H in H2. split.
+      { rewrite <- ctree_eta, H2. eapply t0_det_bind_ret_l; eauto. now left. }
+      left. exists (obs e x), (x0 x), x1. split; auto. rewrite H1. etrans.
+     - exists (CTree.stuckI), (fst r). split.
+       + left. unfold CTree.stuckI. rewrite interp_state_choice.
+         rewrite !choice0_always_stuck. reflexivity.
+       + right. symmetry in H0. apply ret_equ_bind in H0 as (? & ? & ?).
+         exists x. rewrite H. split; etrans. split.
+         rewrite H0. rewrite choice0_always_stuck. etrans.
+         apply interp_state_ret_inv in H0 as []. subst. rewrite H0. destruct r. cbn. apply transis_val. econstructor; etrans.
+Qed.
+
+Lemma trans_interp_state_inv {E F X} (h : E ~> stateT S (ctree F)) (Hh : forall X e s, vsimple (h X e s)) :
+  forall l (t : ctree E X) t' s,
+  trans l (interp_state h t s) t' ->
+  exists l t0 s', t0_det t' (interp_state h t0 s') /\ transi_state h l s s' t t0.
+Proof.
+  intros.
+   assert (trans l (TauI (Ret tt);; interp_state h t s) t').
+   { cbn. etrans. }
+  eapply trans_interp_state_inv_gen in H0; eauto. destruct H0 as (? & ? & ? & ?).
+  destruct H1 as [(? & ? & ? & ? & ? & ?) | (? & ? & ? & ?)].
+  - inv_trans. subst. inv H2. step in H1. inv H1. step in H3. inv H3.
+  - inv_trans. subst. eauto.
+  - left. intros. inv_trans. subst. constructor.
+Qed.
+
+(** The main theorem stating that interp_state preserves sbisim. *)
+
+Theorem interp_state_sbisim_gen {E F X Y} (h : E ~> stateT S (ctree F)) (Hh : forall X e s, vsimple (h X e s)) :
+  forall s (k k' : X -> ctree E Y) (pre pre' : ctree F X),
+  (forall x, sbisim (k x) (k' x)) ->
+  pre ≅ pre' ->
+  vsimple pre ->
+  sbisim (a <- pre;; TauI (interp_state h (k a) s)) (a <- pre';; TauI (interp_state h (k' a) s)).
+Proof.
+  revert X. coinduction R CH.
+  symmetric using idtac.
+  { intros. apply H; eauto.  intros. rewrite H0. reflexivity. now rewrite H1. red; now setoid_rewrite <- H1. }
+  assert (CH' : forall (t t' : ctree E Y) s, t ~ t' -> st R (interp_state h t s) (interp_state h t' s)).
+  {
+    intros.
+    assert (st R (a <- Ret tt;; TauI (interp_state h ((fun _ => t) a) s))
+      (a <- Ret tt;; TauI (interp_state h ((fun _ => t') a) s))).
+    { apply CH; eauto. left; eauto. }
+    setoid_rewrite bind_ret_l in H0.
+    rewrite !sb_tauI in H0.
+    apply H0.
+  }
+  intros. setoid_rewrite <- H0. clear pre' H0. cbn. intros.
+  copy H0. rewrite bind_tau_r in H0.
+  eapply trans_interp_state_inv_gen in H0 as (? & ? & ? & ?); auto.
+  2: { destruct H1 as [[] | []]; rewrite H1.
+    rewrite bind_ret_l. apply is_simple_tauI_ret.
+    rewrite bind_trigger. right. intros. inv_trans. subst.
+    exists x0. rewrite EQ. eright. left. reflexivity. reflexivity.
+  }
+  destruct H2.
+  - destruct H2 as (? & ? & ? & ? & ? & ?). rewrite H4 in H0. clear x H4.
+    destruct H1 as [[] | []].
+    + rewrite H1, bind_ret_l in H2. rewrite H1, bind_ret_l in cpy. inv_trans. subst.
+      inv H3. step in H2. inv H2. step in H4. inv H4.
+    + rewrite H1 in *. rewrite bind_trigger in H2. apply trans_vis_inv in H2 as (? & ? & ?). subst.
+      rewrite H2 in H3. inv H3. step in H4. inv H4.
+      apply equ_choice_invE in H5. 2: apply Fin.F1.
+      rewrite <- H5 in H4. inv H4. 2: { step in H6. inv H6. }
+      step in H3. inv H3. clear x2 H2 t H5.
+      rewrite bind_trigger in cpy. apply trans_vis_inv in cpy. destruct cpy as (? & ? & ?). subst.
+      exists (TauI (interp_state h (k' x1) s)). rewrite H1. rewrite bind_trigger. now constructor.
+      rewrite H2, !sb_tauI. apply CH'. apply H.
+  - destruct H2 as (? & ? & ? & ?).
+    destruct H1 as [[] | []]. 2: { rewrite H1 in H2. setoid_rewrite bind_trigger in H2. inv_trans. }
+    rewrite H1 in *. rewrite bind_ret_l in H2. inv_trans. subst. clear EQ.
+    eapply transis_sbisim in H4; eauto. destruct H4 as (? & ? & ?).
+    apply transis_trans in H2 as (? & ? & ?); auto.
+    exists x3. rewrite H1, bind_ret_l. etrans.
+    assert (st R (interp_state h x x0) (interp_state h x1 x0)).
+    { apply CH'. apply H4. }
+    rewrite sbisim_t0_det. 2: apply H0.
+    setoid_rewrite sbisim_t0_det at 3. 2: apply H5.
+    apply H6.
+Qed.
+
+#[global] Instance interp_state_sbisim {E F R} (h : E ~> stateT S (ctree F)) (Hh : forall X e s, vsimple (h X e s)) :
+  Proper (sbisim ==> eq ==> sbisim) (interp_state h (T := R)).
+Proof.
+  cbn. intros. subst.
+  assert (a <- Ret tt;; TauI (interp_state h ((fun _ => x) a) y0) ~
+    a <- Ret tt;; TauI (interp_state h ((fun _ => y) a) y0)).
+  apply interp_state_sbisim_gen; auto.
+  red; eauto.
+  setoid_rewrite bind_ret_l in H0. rewrite !sb_tauI in H0. apply H0.
+Qed.
 
 End State.
 
